# 微分積分

## Σ計算

```math
\begin{matrix}
\begin{array}{ll}

\sum_{k=1}^{n}k   &= \frac{n(n + 1)}{2}\\
\\
\sum_{k=1}^{n}k^2 &= \frac{n(n + 1)(2n + 1)}{6}\\
\\
\sum_{k=1}^{n}k^3 &= \{\frac{n(n + 1)}{2}\}^2 = \frac{n^2(n + 1)^2}{4}\\
\\
\sum_{k=1}^{n}c   &= nc\\

\end{array}
\end{matrix}
```

## 微分公式


## 積分公式





## 証明

### Σ計算

```math
\begin{matrix}
\begin{array}{ll}

1.&\sum_{k=1}^{n}c   = c + c + c + ... = nc\\
\\
\\
2.\\
&\begin{array}{rll}
   &1  &+ 2     &+ 3     &+ ... &+ n&\\
+) &n  &+ n-1   &+ n-2   &+ ... &+ 1&\\
&---   &----    &----    &---   &----&\\
&(n+1) &+ (n+1) &+ (n+1) &+ ... &+ (n+1) &= (n+1) \cdot n\\
\end{array}\\
&2\sum_{k=1}^{n}k = n(n + 1)\\
\\
&\sum_{k=1}^{n}k = \frac{n(n + 1)}{2}\\
\\
3.\\
&(k+1)^3 - k^3 = 3k^2 + 3k + 1 \\
\\
&\begin{array}{rll}
   &2^3 &-1^3 &= 3\cdot1^2 &+ 3\cdot1 &+ 1\\
   &3^3 &-2^3 &= 3\cdot2^2 &+ 3\cdot2 &+ 1\\
   &4^3 &-3^3 &= 3\cdot3^2 &+ 3\cdot3 &+ 1\\
   &&:&:\\
+) &(n+1)^3 &-n^3 &= 3\cdot n^2 &+ 3\cdot n &+ 1\\
&---   &----    &----    &---   &----&\\
&(n+1)^3 &-1^3 &= 3\sum_{k=1}^{n}k^2 &+ 3\sum_{k=1}^{n}k &+ n\\
\end{array}\\
\\
&\begin{array}{rll}
&3\sum_{k=1}^{n}k^2 &= (n+1)^3 - 1 - n - 3\sum_{k=1}^{n}k\\
& &= (n+1)^3 - (n+1) - 3 \cdot \frac{n(n+1)}{2}\\
& &= \frac{1}{2}(n+1)\{2(n+1)^2 - 2 - 3n\}\\
& &= \frac{1}{2}(n+1)\{2n^2 + n\}\\
& &= \frac{1}{2}n(n+1)(2n + 1)\\
\\
&\sum_{k=1}^{n}k^2 &= \frac{n(n + 1)(2n + 1)}{6}\\
\end{array}\\
\\
\\
4.\\
&(k+1)^4 - k^4 = 4k^3 + 6k^2 + 4k + 1 \\
\\
&\begin{array}{rll}
   &2^4 &-1^4 &= 4\cdot1^3 &+ 6\cdot1^2 &+ 4\cdot1 &+ 1\\
   &3^4 &-2^4 &= 4\cdot2^3 &+ 6\cdot2^2 &+ 4\cdot2 &+ 1\\
   &4^4 &-3^4 &= 4\cdot3^3 &+ 6\cdot3^2 &+ 4\cdot3 &+ 1\\
   &&:&:\\
+) &(n+1)^4 &-n^4 &= 4\cdot n^3 &+ 6\cdot n^2 &+ 4\cdot n &+ 1\\
&---   &----    &----    &---   &----&\\
&(n+1)^4 &-1^4 &= 4\sum_{k=1}^{n}k^3 &+ 6\sum_{k=1}^{n}k^2 &+ 4\sum_{k=1}^{n}k &+ n\\
\end{array}\\
\\
&\begin{array}{rll}
&4\sum_{k=1}^{n}k^3 &= (n+1)^4 - 1 - n - 6\sum_{k=1}^{n}k^2 - 4\sum_{k=1}^{n}k\\
& &= (n+1)^4 - (n+1) - 6 \cdot \frac{n(n+1)(2n+1)}{6} - 4 \cdot \frac{n(n+1)}{2}\\
& &= (n+1)\{(n+1)^3 - 1 - n(2n+1) - 2n\}\\
& &= (n+1)\{(n+1)^3 - (2n^2 +3n +1)\}\\
& &= (n+1)\{(n+1)^3 - (2n+1)(n+1)\}\\
& &= (n+1)^2\{(n+1)^2 - (2n+1)\}\\
& &= n^2(n+1)^2\\
\\
&\sum_{k=1}^{n}k^3 &= \frac{n^2(n + 1))^2}{4} = \{\frac{n(n+1)}{2}\}^2\\
\end{array}\\

\end{array}
\end{matrix}
```






